update exponentiation

src/Rupicola/Examples/ECC/Exponentiation.v
@@ -43,34 +43,34 @@ Section S.
     Lemma mod_exp :
       forall m, m <> 0 -> forall b a, ((a mod m) ^ Zpos b) mod m = (a ^ Zpos b) mod m.
     Proof.
-    induction b; intros.
-    - rewrite Pos2Z.pos_xI.
-      rewrite Z.pow_add_r by lia.
-      rewrite Z.pow_1_r.
-      rewrite Z.pow_twice_r.
-      rewrite <- Z.mul_mod_idemp_l by assumption.
-      remember (((a mod m) ^ Z.pos b * (a mod m) ^ Z.pos b) mod m) as A.
-      rewrite Z.mul_mod_idemp_r by assumption.
-      rewrite Z.mul_mod in HeqA by assumption.
-      rewrite IHb in HeqA.
-      rewrite <- Z.mul_mod in HeqA by assumption.
-      rewrite HeqA.
-      rewrite Z.mul_mod_idemp_l by assumption.
-      apply mod_equal.
-      rewrite Z.pow_add_r by lia.
-      rewrite Z.pow_twice_r.
-      lia.
-    - rewrite Pos2Z.pos_xO.
-      rewrite Z.pow_twice_r.
-      rewrite Z.mul_mod by assumption.
-      rewrite IHb.
-      rewrite <- Z.mul_mod by assumption.
-      apply mod_equal.
-      rewrite Z.pow_twice_r.
-      reflexivity.
-    - repeat rewrite Z.pow_1_r.
-      rewrite Z.mod_mod by assumption.
-      reflexivity.
+      induction b; intros.
+      - rewrite Pos2Z.pos_xI.
+        rewrite Z.pow_add_r by lia.
+        rewrite Z.pow_1_r.
+        rewrite Z.pow_twice_r.
+        rewrite <- Z.mul_mod_idemp_l by assumption.
+        remember (((a mod m) ^ Z.pos b * (a mod m) ^ Z.pos b) mod m) as A.
+        rewrite Z.mul_mod_idemp_r by assumption.
+        rewrite Z.mul_mod in HeqA by assumption.
+        rewrite IHb in HeqA.
+        rewrite <- Z.mul_mod in HeqA by assumption.
+        rewrite HeqA.
+        rewrite Z.mul_mod_idemp_l by assumption.
+        apply mod_equal.
+        rewrite Z.pow_add_r by lia.
+        rewrite Z.pow_twice_r.
+        lia.
+      - rewrite Pos2Z.pos_xO.
+        rewrite Z.pow_twice_r.
+        rewrite Z.mul_mod by assumption.
+        rewrite IHb.
+        rewrite <- Z.mul_mod by assumption.
+        apply mod_equal.
+        rewrite Z.pow_twice_r.
+        reflexivity.
+      - repeat rewrite Z.pow_1_r.
+        rewrite Z.mod_mod by assumption.
+        reflexivity.
     Qed.
 
     Fixpoint exp_by_squaring (x : Z) (n : positive) : Z :=
@@ -82,6 +82,22 @@ Section S.
                  x * res
       end.
 
+    Definition inplace {A : Type} (x : A) : A :=
+      x.
+    
+    Arguments inplace : simpl never.
+
+    Fixpoint exp_by_squaring' (x : Z) (n : positive) : Z :=
+      match n with
+      | xH => x mod M
+      | xO xH => x^2 mod M
+      | xI xH => let/d res := x^2 in x * res
+      | xO n' => let/d res := exp_by_squaring' x n' in inplace(res^2)
+      | xI n' => let/d res := exp_by_squaring' x n' in
+                 let/d res := inplace(res^2) in
+                 (x * inplace(res))
+      end.
+
     Lemma let_equal :
       forall A B (val : A) (body_l body_r : A -> B),
         (let x := val in body_l x = body_r x)
@@ -91,34 +107,54 @@ Section S.
     Qed.
 
     Lemma let_nested :
-      forall A (a : A) (val1 : A) (body1 body2 : A -> A),
+      forall A B C (a : C) (val1 : A) (body1 : A -> B) (body2 : B -> C),
         a = (let/d x := val1 in let/d y := body1 x in body2 y)
         -> a = (let/d y := let/d x := val1 in body1 x in body2 y).
     Proof.
       intros. assumption.
     Qed.
+    
+    Lemma let_paren_equal :
+      forall A B (a : A) (val : A) (body_r : A -> B) left,
+        left = (let/d y:= val in (a, body_r y))
+        -> left = (a, let/d y := val in body_r y).
+    Proof.
+      intros. unfold dlet.
+      rewrite H. reflexivity.
+    Qed.
 
     Ltac tac :=
-      intros;
       match goal with
+      | [ |- let _ := _ in _ = _ ] =>
+        intros
       | [ |- _ = let/d _ := let/d _ := _ in _ in _] =>
         eapply let_nested
-      | [ |- _ = let/d x := _ in _] =>
+      | [ |- _ = let/d _ := _ in _] =>
         eapply let_equal with (body_l := fun _ => _)
+      | [ |- _ = (_, let/d _ := _ in _)] =>
+        eapply let_paren_equal
       end.
 
-    Lemma rewrite :
-      {rewritten : Z -> Z & forall x, rewritten x = exp_by_squaring x 11}.
-    Proof.
-      cbv beta delta [exp_by_squaring].
-      eexists.
-      repeat tac.
-      reflexivity.
+    Derive rewritten' SuchThat
+           (forall x, rewritten' x = exp_by_squaring x 11)
+           As rewrite'.
+    cbv beta iota delta [exp_by_squaring].
+    subst rewritten'.
+    intros.
+    repeat tac.
+    reflexivity.
     Defined.
+    Print rewritten'.
 
-    Definition rewritten :=
-      Eval simpl in projT1 (rewrite).
-
+    Derive rewritten SuchThat
+           (forall x, rewritten x = (x, let/d res := exp_by_squaring' x 11 in res))
+           As rewrite.
+    cbv beta iota delta [exp_by_squaring'].
+    subst rewritten.
+    intros.
+    repeat tac.
+    reflexivity.
+    Defined.
     Print rewritten.
 
     Lemma exp_by_squaring_correct :
@@ -153,7 +189,7 @@ Section S.
        (["x"; "sq"], [],
         bedrock_func_body:
           (
-            cmd.call [] bignum_copy [expr.var "sq"; expr.var "x"];;
+            cmd.call [] bignum_copy [expr.var "x"; expr.var "sq"];;
             cmd.call [] square [expr.var "sq"; expr.var "sq"];;
             cmd.call [] mul [expr.var "x"; expr.var "sq"; expr.var "sq"];;
             cmd.call [] square [expr.var "sq"; expr.var "sq"]
@@ -161,8 +197,540 @@ Section S.
        )
       ).
 
+    Instance spec_of_exp_6 : spec_of exp_6 :=
+      fun functions =>
+        forall x_ptr x x_val sq_ptr sq ret tr R mem,
+          bounded_by tight_bounds sq ->
+          bounded_by tight_bounds x ->
+          bounded_by tight_bounds ret ->
+          exp_by_squaring_6 x_val = eval ret ->
+          ((Bignum x_ptr x * Bignum sq_ptr sq * R)%sep mem) ->
+          x_val = eval x ->
+          WeakestPrecondition.call
+            functions exp_6 tr mem [x_ptr; sq_ptr]
+            (fun tr' mem' rets =>
+               tr = tr' /\ rets = nil
+               /\ (Bignum x_ptr x * Bignum sq_ptr ret * R)%sep mem').
 
+    Ltac tac :=
+      repeat match goal with
+             | [ |- WeakestPrecondition.dexprs _ _ _ _ ] => eexists
+             | [ |- WeakestPrecondition.list_map _ _ _ ] => eexists
+             | [ |- _ /\ _] => split
+             | _ => reflexivity
+             | [ |- context[map.get (map.put _ ?k _) ?k] ] => rewrite map.get_put_same
+             | [ |- context[map.get (map.put _ ?k _) ?k2] ] => rewrite map.get_put_diff by discriminate
+             | [ |- WeakestPrecondition.call _ _ _ _ _ _ ] => handle_call
+             | [ |- bounded_by loose_bounds ?x ] => eapply relax_bounds
+             | [ H : bounded_by tight_bounds ?x |- bounded_by tight_bounds ?x] => apply H
+             | [ |- exists _, _ ] => eexists
+             | [ H : context[emp (?k = [])] |- context[map.putmany_of_list_zip [] ?k] ] => destruct H
+             | [ H : ?k = [] |- context[map.putmany_of_list_zip [] ?k] ] => rewrite H
+             | [ |- WeakestPrecondition.cmd _ _ _ _ _ _ ] => straightline
+             | [ |- WeakestPrecondition.call _ _ _ _ _ ] => handle_call
+             | [ |- WeakestPrecondition.call _ _ _ _ _ ] => straightline_call
+             | [ H : context[postcondition_func_norets] |- _ ] => destruct H
+             end.
+    
+    
+    Lemma exp_6_correct : program_logic_goal_for_function! exp_6.
+    Proof.
+      repeat straightline.
+      intros; exists [x_ptr; sq_ptr]; split.
+      - subst l. tac.
+      - subst l. tac.
+        Print spec_of_mul.
+        straightline_call; destruct_lists_of_known_length. 
+        + split.
+          2: { split.
+               2: { admit. }
+               admit.
+          }
+          admit.
+        + admit.
+          Unshelve.
+          { exact x. }
+          { exact x. }
+          { exact R. }
+          exact x.
+    Admitted.
 
+    Definition exp_result x_ptr q_ptr xq_val : list word -> Semantics.mem -> Prop :=
+      fun _ => Lift1Prop.ex1 (fun x => Lift1Prop.ex1 (fun q =>
+                                                        (emp(eval x = fst xq_val) *
+                                                         (emp(eval q mod M = snd xq_val) *
+                                                          (Bignum x_ptr x * Bignum q_ptr q)))%sep)).
+
+    Definition exp_by_squaring_6' (x : Z) : (Z * Z) :=
+      let/d x2 := x ^ 2 mod M in
+      let/d x3 := x2 * x mod M in
+      let/d x6 := x3 ^ 2 mod M in
+      (x, x6).
+
+    Lemma Lift1Prop_impl1_ex :
+      forall {A B : Type} (q : A -> B -> Prop) (p : A -> Prop),
+        (exists v, (Lift1Prop.impl1 p (fun m => q m v))) ->
+        Lift1Prop.impl1 p (fun m => exists v, q m v).
+      intros.
+      unfold Lift1Prop.impl1.
+      unfold Lift1Prop.impl1 in H.
+      intros.
+      destruct H.
+      exists x0.
+      apply H.
+      apply H0.
+    Qed.
+    
+    Lemma Lift1Prop_impl1_and :
+      forall {A : Type} (q1 : Prop) (q2 p : A -> Prop),
+        (q1 /\ (Lift1Prop.impl1 p (fun m => q2 m))) ->
+        Lift1Prop.impl1 p (fun m => q1 /\ q2 m).
+      intros.
+      unfold Lift1Prop.impl1.
+      unfold Lift1Prop.impl1 in H.
+      intros.
+      destruct H.
+      split.
+      - apply H.
+      - apply H1.
+        apply H0.
+    Qed.
+    
+    Derive exp_body SuchThat
+           (let exp6 := ("exp6", (["x"; "sq"], [], exp_body)) in
+            program_logic_goal_for exp6
+                                   (forall functions,
+                                       spec_of_square functions ->
+                                       spec_of_mul functions ->
+                                       forall x_ptr x sq_ptr sq_init tr R mem,
+                                         bounded_by tight_bounds x ->
+                                         bounded_by tight_bounds sq_init ->
+                                         ((Bignum x_ptr x * Placeholder sq_ptr sq_init * R)%sep mem) ->
+                                         WeakestPrecondition.call
+                                           (exp6 :: functions)
+                                           "exp6"
+                                           tr mem [x_ptr; sq_ptr]
+                                           (postcondition_func_norets
+                                              (exp_result x_ptr sq_ptr (exp_by_squaring_6' (eval x)))
+                                              R tr)))
+           As exp_body_correct.
+    Proof.
+      cbv[program_logic_goal_for].
+      intros.
+      WeakestPrecondition.unfold1_call_goal.
+      cbv beta match delta [WeakestPrecondition.call_body].
+                     lazymatch goal with
+                     | |- if ?test then ?T else _ => replace test with true by reflexivity; change T
+                     end.
+                     cbv beta match delta [WeakestPrecondition.func].
+                                    repeat straightline.
+                                    subst_lets_in_goal.
+                                    apply postcondition_func_norets_postcondition_cmd.
+                                    unfold exp_by_squaring_6'.
+                                    eapply compile_square; eauto; try compile_step.
+                                    Z.push_mod.
+                                    rewrite Zmod_mod.
+                                    Z.pull_mod.
+                                    eapply compile_mul; eauto; try compile_step.
+                                    rewrite <- Z.pow_mod.
+                                    eapply compile_square; eauto; try compile_step.
+                                    compile_done.
+                                    unfold exp_result.
+                                    unfold fst.
+                                    unfold snd.
+                                    apply sep_comm.
+                                    assert ((R * (Bignum x_ptr x  * Bignum sq_ptr out1))%sep m1) as Hsep by ecancel_assumption.
+                                    revert Hsep.
+                                    eapply Proper_sep_impl1.
+                                    - reflexivity.
+                                    - apply Lift1Prop_impl1_ex. exists x.
+                                      apply Lift1Prop_impl1_ex. exists out1.
+                                      eapply impl1_r_sep_emp.
+                                      split; try reflexivity.
+                                      eapply impl1_r_sep_emp.
+                                      split; try reflexivity.
+    Qed.
+
+    Definition exp_by_squaring_9' (x : Z) : (Z * Z) :=
+      let/d sq := x ^ 2 mod M in
+      let/d sq := sq ^ 2 mod M in
+      let/d sq := sq ^ 2 mod M in
+      let/d sq := x * sq mod M in
+      (x, sq).
+
+    Ltac compile_custom ::=
+      match goal with
+      | [ |- find _ implementing exp_result _ _ (let/d _ := eval _ ^ 2 mod M in _) and-returning _ and-locals-post _ with-locals _ and-memory _ and-trace _ and-rest _ and-functions _] => eapply compile_square; eauto; try compile_step
+      | [ |- find _ implementing exp_result _ _ (let/d _ := (eval _ * eval _) mod M in _) and-returning _ and-locals-post _ with-locals _ and-memory _ and-trace _ and-rest _ and-functions _] => eapply compile_mul; eauto; try compile_step
+      | [ |- find _ implementing exp_result _ _ (let/d _ := (eval _ mod M) ^ 2 mod M in _) and-returning _ and-locals-post _ with-locals _ and-memory _ and-trace _ and-rest _ and-functions _] => rewrite <- Z.pow_mod
+      | [ |- find _ implementing exp_result _ _ (let/d _ := (eval _ mod M *  _) mod M in _) and-returning _ and-locals-post _ with-locals _ and-memory _ and-trace _ and-rest _ and-functions _] => rewrite Zmult_mod_idemp_l
+      | [ |- find _ implementing exp_result _ _ (let/d _ := ( _ * (eval _ mod M)) mod M in _) and-returning _ and-locals-post _ with-locals _ and-memory _ and-trace _ and-rest _ and-functions _] => rewrite Zmult_mod_idemp_r
+      end.
+
+    Hint Unfold exp_result : compiler.
+    
+    Derive exp9_body SuchThat
+           (let exp9 := ("exp9", (["x"; "sq"], [], exp9_body)) in
+            program_logic_goal_for exp9
+                                   (forall functions,
+                                       spec_of_square functions ->
+                                       spec_of_mul functions ->
+                                       forall x_ptr x sq_ptr sq_init tr R mem,
+                                         bounded_by tight_bounds x ->
+                                         bounded_by tight_bounds sq_init ->
+                                         ((Bignum x_ptr x * Placeholder sq_ptr sq_init * R)%sep mem) ->
+                                         WeakestPrecondition.call
+                                           (exp9 :: functions)
+                                           "exp9"
+                                           tr mem [x_ptr; sq_ptr]
+                                           (postcondition_func_norets
+                                              (exp_result x_ptr sq_ptr (exp_by_squaring_9' (eval x)))
+                                              R tr)))
+           As exp9_body_correct.
+    Proof.
+      compile.
+      autounfold with compiler.
+      cbn.
+      apply sep_comm.
+      match goal with
+      | [ H : (Bignum sq_ptr ?sq * (Bignum x_ptr ?x * ?R))%sep ?m |- _ ?m ] =>
+        assert (((R * (Bignum x_ptr x * Bignum sq_ptr sq)))%sep m) as Hsep by ecancel_assumption
+      end.
+      revert Hsep.
+      eapply Proper_sep_impl1.
+      - reflexivity.
+      - apply Lift1Prop_impl1_ex. eexists.
+        apply Lift1Prop_impl1_ex. eexists.
+        eapply impl1_r_sep_emp.
+        split; try reflexivity.
+        eapply impl1_r_sep_emp.
+        split; try reflexivity.
+    Qed.
+    
+    Lemma compile_square_inplace :
+      forall (locals: Semantics.locals) (mem: Semantics.mem)
+             (locals_ok : Semantics.locals -> Prop)
+             tr retvars R Rin functions T
+             (pred: T -> list word -> Semantics.mem -> Prop)
+             (x : bignum) x_ptr x_var k k_impl,
+        spec_of_square functions ->
+        bounded_by loose_bounds x ->
+        (Bignum x_ptr x * Rin)%sep mem ->
+        map.get locals x_var = Some x_ptr ->
+        let v := (eval x ^ 2) mod M in
+        (let head := v in
+         forall out m,
+           eval out mod M = head ->
+           bounded_by tight_bounds out ->
+           sep (Bignum x_ptr out) Rin m ->
+           (find k_impl
+                 implementing (pred (k (eval out mod M)))
+                 and-returning retvars
+                               and-locals-post locals_ok
+            with-locals locals and-memory m and-trace tr and-rest R
+                                                                  and-functions functions)) ->
+        (let head := inplace(v) in
+         find (cmd.seq
+                 (cmd.call [] square [expr.var x_var; expr.var x_var])
+                 k_impl)
+              implementing (pred (dlet head k))
+              and-returning retvars
+                            and-locals-post locals_ok
+         with-locals locals and-memory mem and-trace tr and-rest R
+                                                                 and-functions functions).
+    Proof.
+      intros.
+      eapply compile_square; eauto.
+    Qed.
+
+    Lemma compile_square_sep :
+      forall (locals: Semantics.locals) (mem: Semantics.mem)
+             (locals_ok : Semantics.locals -> Prop)
+             tr retvars R Rin functions T
+             (pred: T -> list word -> Semantics.mem -> Prop)
+             (x out1 : bignum) x_ptr x_var out_ptr out_var k k_impl,
+        spec_of_square functions ->
+        bounded_by loose_bounds x ->
+        (Bignum x_ptr x * Bignum out_ptr out1 * Rin)%sep mem ->
+        map.get locals x_var = Some x_ptr ->
+        map.get locals out_var = Some out_ptr ->
+        let v := (eval x ^ 2) mod M in
+        (let head := v in
+         forall out m,
+           eval out mod M = head ->
+           bounded_by tight_bounds out ->
+           (Bignum x_ptr x * Bignum out_ptr out * Rin)%sep m ->
+           (find k_impl
+                 implementing (pred (k (eval out mod M)))
+                 and-returning retvars
+                               and-locals-post locals_ok
+            with-locals locals and-memory m and-trace tr and-rest R
+                                                                  and-functions functions)) ->
+        (let head := v in
+         find (cmd.seq
+                 (cmd.call [] square [expr.var x_var; expr.var out_var])
+                 k_impl)
+              implementing (pred (dlet head k))
+              and-returning retvars
+                            and-locals-post locals_ok
+         with-locals locals and-memory mem and-trace tr and-rest R
+                                                                 and-functions functions).
+    Proof.
+      intros.
+      eapply compile_square; eauto.
+      - ecancel_assumption.
+      - unfold Placeholder. ecancel_assumption.
+      - intros. apply H4; eauto. ecancel_assumption.
+    Qed.
+
+    Lemma compile_mul_inplace_right :
+      forall (locals: Semantics.locals) (mem: Semantics.mem)
+             (locals_ok : Semantics.locals -> Prop)
+             tr retvars R Rin functions T
+             (pred: T -> list word -> Semantics.mem -> Prop)
+             (x y : bignum) x_ptr x_var y_ptr y_var k k_impl,
+        spec_of_mul functions ->
+        bounded_by loose_bounds x ->
+        bounded_by loose_bounds y ->
+        (Bignum x_ptr x * Bignum y_ptr y * Rin)%sep mem ->
+        map.get locals x_var = Some x_ptr ->
+        map.get locals y_var = Some y_ptr ->
+        let v := (eval x * eval y) mod M in
+        (let head := v in
+         forall out m,
+           eval out mod M = head ->
+           bounded_by tight_bounds out ->
+           (Bignum x_ptr x * Bignum y_ptr out * Rin)%sep m ->
+           (find k_impl
+                 implementing (pred (k (eval out mod M)))
+                 and-returning retvars
+                               and-locals-post locals_ok
+            with-locals locals and-memory m and-trace tr and-rest R
+                                                                  and-functions functions)) ->
+        (let head := v in
+         find (cmd.seq
+                 (cmd.call [] mul [expr.var x_var; expr.var y_var;
+                                  expr.var y_var])
+                 k_impl)
+              implementing (pred (dlet head k))
+              and-returning retvars
+                            and-locals-post locals_ok
+         with-locals locals and-memory mem and-trace tr and-rest R
+                                                                 and-functions functions).
+    Proof.
+      intros.
+      eapply compile_mul; eauto; try ecancel_assumption.
+      - unfold Placeholder. ecancel_assumption.
+      - intros. apply H5; eauto. ecancel_assumption.
+    Qed.
+
+    Lemma compile_mul_sep :
+      forall (locals: Semantics.locals) (mem: Semantics.mem)
+             (locals_ok : Semantics.locals -> Prop)
+             tr retvars R Rin functions T
+             (pred: T -> list word -> Semantics.mem -> Prop)
+             (x y out1 : bignum) x_ptr x_var y_ptr y_var out_ptr out_var k k_impl,
+        spec_of_mul functions ->
+        bounded_by loose_bounds x ->
+        bounded_by loose_bounds y ->
+        (Bignum x_ptr x * Bignum y_ptr y * Bignum out_ptr out1 * Rin)%sep mem ->
+        map.get locals x_var = Some x_ptr ->
+        map.get locals y_var = Some y_ptr ->
+        map.get locals out_var = Some out_ptr ->
+        let v := (eval x * eval y) mod M in
+        (let head := v in
+         forall out m,
+           eval out mod M = head ->
+           bounded_by tight_bounds out ->
+           (Bignum x_ptr x * Bignum y_ptr y * Bignum out_ptr out * Rin)%sep m ->
+           (find k_impl
+                 implementing (pred (k (eval out mod M)))
+                 and-returning retvars
+                               and-locals-post locals_ok
+            with-locals locals and-memory m and-trace tr and-rest R
+                                                                  and-functions functions)) ->
+        (let head := v in
+         find (cmd.seq
+                 (cmd.call [] mul [expr.var x_var; expr.var y_var;
+                                  expr.var out_var])
+                 k_impl)
+              implementing (pred (dlet head k))
+              and-returning retvars
+                            and-locals-post locals_ok
+         with-locals locals and-memory mem and-trace tr and-rest R
+                                                                 and-functions functions).
+    Proof.
+      intros.
+      eapply compile_mul; eauto; try ecancel_assumption.
+      - unfold Placeholder. ecancel_assumption.
+      - intros. apply H6; eauto. ecancel_assumption.
+    Qed.
+
+    Lemma Zmult_mod_idemp_r_inplace :
+      forall a b n : Z,
+        (b * inplace (a mod n)) mod n = (b * inplace(a)) mod n.
+      unfold inplace.
+      apply Zmult_mod_idemp_r.
+    Qed.
+
+    Ltac compile_custom ::=
+      match goal with
+      | [ |- find _ implementing exp_result _ _ (let/d _ := eval _ ^ 2 mod M in _) and-returning _ and-locals-post _ with-locals _ and-memory _ and-trace _ and-rest _ and-functions _] => eapply compile_square_sep; eauto; try compile_step
+      | [ |- find _ implementing exp_result _ _ (let/d _ := inplace (eval _ ^ 2 mod M) in _) and-returning _ and-locals-post _ with-locals _ and-memory _ and-trace _ and-rest _ and-functions _] => eapply compile_square_inplace; eauto; try compile_step
+      | [ |- find _ implementing exp_result _ _ (let/d _ := (eval _ * eval _) mod M in _) and-returning _ and-locals-post _ with-locals _ and-memory _ and-trace _ and-rest _ and-functions _] => eapply compile_mul_sep; eauto; try compile_step
+      | [ |- find _ implementing exp_result _ _ (let/d _ := (eval _ * inplace (eval _) mod M) in _) and-returning _ and-locals-post _ with-locals _ and-memory _ and-trace _ and-rest _ and-functions _] => eapply compile_mul_inplace_right; eauto; try compile_step
+      | [ |- find _ implementing exp_result _ _ (let/d _ := (eval _ mod M) ^ 2 mod M in _) and-returning _ and-locals-post _ with-locals _ and-memory _ and-trace _ and-rest _ and-functions _] => rewrite <- Z.pow_mod
+      | [ |- find _ implementing exp_result _ _ (let/d _ := inplace ((eval _ mod M) ^ 2 mod M) in _) and-returning _ and-locals-post _ with-locals _ and-memory _ and-trace _ and-rest _ and-functions _] => rewrite <- Z.pow_mod
+      | [ |- find _ implementing exp_result _ _ (let/d _ := (eval _ mod M *  _) mod M in _) and-returning _ and-locals-post _ with-locals _ and-memory _ and-trace _ and-rest _ and-functions _] => rewrite Zmult_mod_idemp_l
+      | [ |- find _ implementing exp_result _ _ (let/d _ := ( _ * (eval _ mod M)) mod M in _) and-returning _ and-locals-post _ with-locals _ and-memory _ and-trace _ and-rest _ and-functions _] => rewrite Zmult_mod_idemp_r
+      | [ |- find _ implementing exp_result _ _ (let/d _ := ( _ * inplace (eval _ mod M)) mod M in _) and-returning _ and-locals-post _ with-locals _ and-memory _ and-trace _ and-rest _ and-functions _] => rewrite Zmult_mod_idemp_r_inplace
+      | [ |- find _ implementing exp_result _ _ (let/d _ := inplace (( _ * (eval _ mod M)) mod M) in _) and-returning _ and-locals-post _ with-locals _ and-memory _ and-trace _ and-rest _ and-functions _] => rewrite Zmult_mod_idemp_r
+      end.
+    
+    Derive exp_11_body SuchThat
+           (let exp11 := ("exp11", (["x"; "sq"], [], exp_11_body)) in
+            program_logic_goal_for exp11
+                                   (forall functions,
+                                       spec_of_square functions ->
+                                       spec_of_mul functions ->
+                                       forall x_ptr x sq_ptr sq_init tr R mem,
+                                         bounded_by tight_bounds x ->
+                                         bounded_by tight_bounds sq_init ->
+                                         ((Bignum x_ptr x * Placeholder sq_ptr sq_init * R)%sep mem) ->
+                                         WeakestPrecondition.call
+                                           (exp11 :: functions)
+                                           "exp11"
+                                           tr mem [x_ptr; sq_ptr]
+                                           (postcondition_func_norets
+                                              (exp_result x_ptr sq_ptr (rewritten (eval x)))
+
+                                              R tr)))
+           As exp_11_body_correct.
+    Proof.
+      compile.
+      autounfold with compiler.
+      cbn.
+      apply sep_comm.
+      match goal with
+      | [ H : (Bignum x_ptr ?x * Bignum sq_ptr ?sq * ?R)%sep ?m |- _ ?m ] =>
+        assert (((R * (Bignum x_ptr x * Bignum sq_ptr sq)))%sep m) as Hsep by ecancel_assumption
+      end.
+      revert Hsep.
+      eapply Proper_sep_impl1.
+      - reflexivity.
+      - apply Lift1Prop_impl1_ex. eexists.
+        apply Lift1Prop_impl1_ex. eexists.
+        eapply impl1_r_sep_emp.
+        split; try reflexivity.
+        eapply impl1_r_sep_emp.
+        split; try reflexivity.
+    Qed.
+
+    Fixpoint run_length_encoding (n : positive) : list (bool * nat) :=
+      match n with
+      | xH => [(true, 0)]
+      | xO n' =>
+        match (run_length_encoding n') with
+        | (false, k) :: t => (false, k + 1) :: t
+        | t => (false, 0) :: t
+        end
+      | xI n' =>
+        match (run_length_encoding n') with
+        | (true, k) :: t => (true, k + 1) :: t
+        | t => (true, 0) :: t
+        end
+      end%nat.
+
+    Compute run_length_encoding 1.
+
+    (*Fixpoint loop_square (x : Z) (k : nat) : Z :=
+       match k with
+       | 0%nat => x mod M
+       | 1%nat => x^2 mod M
+       | S k' => let/d res := (loop_square x k') in
+                       inplace(res^2)
+       end.*)
+
+    Fixpoint loop {A} (x : A) (k : nat) (f : A -> A) : A :=
+      match k with
+      | 0%nat => f x
+      | S k' => f (loop x k' f)
+      end.
+
+    Definition exp_square_and_multiply (x : Z) (x' : Z) :=
+      (Z.pow x' 2 mod M) * x mod M.
+
+    Definition exp_square (x' : Z) :=
+      (Z.pow x' 2 mod M).
+
+    Fixpoint exp_from_encoding (x : Z) (n : list (bool * nat)) : Z :=
+      match n with
+      | [] =>
+        1
+      (* can add more cases for small k to be faster *)
+      | (true, 0%nat) :: t =>
+        let/d res := exp_from_encoding x t in
+        let/d res := inplace(res^2 mod M) in
+        let/d res := x * inplace(res) mod M in
+        res
+      | (true, k) :: t =>
+        let/d res := exp_from_encoding x t in
+        let/d res := loop res k (exp_square_and_multiply x) in
+        res
+      | (false, 0%nat) :: t =>
+        let/d res := exp_from_encoding x t in
+        let/d res := res^2 mod M in
+        res
+      | (false, k) :: t =>
+        let/d res := exp_from_encoding x t in
+        let/d res := loop res k (exp_square) in
+        res
+      end.
+
+    Definition exp_by_squaring_encoded (x : Z) (n : positive) : Z :=
+      exp_from_encoding x (run_length_encoding n).
+
+    Compute run_length_encoding 4.
+
+    Lemma exp_by_squaring_encoded_correct :
+      M <> 0 -> forall n x, exp_by_squaring_encoded x n = x ^ (Zpos n) mod M.
+    Proof.
+      intros. rewrite <- exp_by_squaring_correct; eauto.
+      unfold exp_by_squaring_encoded; induction n; simpl.
+      - cbn -[loop].
+        destruct (run_length_encoding n).
+        + rewrite <- IHn. eauto.
+        + destruct p. destruct b.
+          { rewrite <- IHn.
+          cbn. replace (n0 + 1)%nat with (S n0).
+          { unfold dlet; unfold inplace; destruct n0.
+            { cbn.
+              repeat eapply mod_equal.
+              rewrite <- Z.mul_comm.
+              f_equal.
+              eapply mod_equal.
+              set ((exp_from_encoding x l)) as exl.
+              ring_simplify.
+              rewrite <- Z.mul_comm. reflexivity.
+            }
+            eapply mod_equal.
+            eapply Z.mul_comm.
+          }
+          { symmetry. eapply Nat.add_1_r. }
+          }
+        rewrite <- IHn. cbn. unfold dlet; unfold inplace. eauto.
+      - rewrite <- IHn.
+        cbn.
+        unfold dlet.
+        destruct (run_length_encoding n) as [|[[|] n0] t]; eauto.
+        rewrite Nat.add_comm.
+        destruct n0; eauto.
+      - unfold dlet; unfold inplace; cbn.
+        rewrite Zmult_mod_idemp_r.
+        eapply mod_equal.
+        apply Z.mul_1_r.
+    Qed.
+    
   End Bedrock.
 
 End S.
